LeanPy/Data/Object/Id.lean
@@ -3,6 +3,7 @@ Copyright (c) 2025 Mac Malone. All rights reserved.
 Released under the Apache 2.0 license as described in the file LICENSE.
 syntax Authors Mac Malone
 -/
+import LeanPy.Data.IntRef
 import LeanPy.Util.String
 
 namespace LeanPy
@@ -10,32 +11,79 @@ namespace LeanPy
 /--
 The type of Python object ids.
 
-Unlike CPython, object identities in LeanPy are not derived from the object's
-address. Instead, LeanPy uses a mix of methods to determine an identifier for
-an object.
+Unlike CPython, object identities in LeanPy are not solely derived from
+the object's address. Instead, LeanPy uses a mix of methods to determine
+the identifier for an object.
 
 For unique constants (e.g., `None`, `False`, `True`, `Ellipsis`,
-`NoteImplemented`), a fixed id is used. For small integers, their
+`NotImplemented`), a fixed constant id is used. For small integers, their
 scalar value is used. For big integers and other objects with a non-scalar
 Lean representation, their address is used.
 -/
 structure ObjectId where
-  val : UInt64
-  deriving Nonempty, BEq
+  private mk ::
+    private val : UInt64
+  deriving Nonempty, DecidableEq, Hashable
 
 namespace ObjectId
 
-def hex (self : ObjectId) : String :=
+def toNat (self : ObjectId) : Nat :=
+  self.val.toNat
+
+@[simp] theorem toNat_mk : toNat (mk n) = n.toNat := rfl
+
+theorem toNat.inj : toNat n = toNat m → n = m := by
+  cases n; cases m; simp [toNat, UInt64.toNat_inj]
+
+theorem toNat_inj : toNat n = toNat m ↔ n = m :=
+  .intro toNat.inj (congrArg toNat)
+
+@[inline] def hex (self : ObjectId) : String :=
   upperHexUInt64 self.val
 
-def none : ObjectId := .mk 0
-def false : ObjectId := .mk <| 2 ^ 32
-def true : ObjectId := .mk <| 2 ^ 32 + 1
-def ellipsis : ObjectId := .mk <| 2 ^ 32 + 2
-def notImplemented : ObjectId := .mk <| 2 ^ 32 + 3
+instance : ToString ObjectId := ⟨ObjectId.hex⟩
 
-def int (n : Int) : ObjectId :=
-  .mk <| (unsafe ptrAddrUnsafe n).toUInt64
+def const (n : UInt8) : ObjectId :=
+  ⟨(n.toUInt64 + 1) <<< 33 ||| 1⟩
+
+private theorem toNat_const : toNat (const n)  = (n.toNat + 1) * 2 ^ 33 + 1 := by
+  have eq_add_one {n : Nat} (h : n % 2 = 0) : n ||| 1 = n + 1 :=
+    Nat.eq_of_testBit_eq fun
+    | 0 => by simp [Nat.add_mod, h]
+    | i+1 => by simp [↓Nat.testBit_or, Nat.testBit_add_one, Nat.add_div, h]
+  have n_lt : n.toNat < 256 := n.toNat_lt
+  have h1 : n.toNat + 1 < 18446744073709551616 := by omega
+  have h2 : (n.toNat + 1) * 8589934592 < 18446744073709551616 := by omega
+  have h3 : (n.toNat + 1) * 8589934592 % 2 = 0 := by omega
+  simp [const, Nat.mod_eq_of_lt h1, Nat.shiftLeft_eq, Nat.mod_eq_of_lt h2, eq_add_one h3]
+
+@[simp] private theorem toNat_const_mod_two : toNat (const n) % 2 = 1 := by
+  simp [const]
+
+private theorem le_toNat_const : 8589934592 ≤ toNat (const n) := by
+  simp only [toNat_const, Nat.reducePow, Nat.reduceLeDiff]
+  exact Nat.le_trans (by simp) (Nat.le_mul_of_pos_left 8589934592 (by simp))
+
+def none : ObjectId := const 0
+def false : ObjectId := const 1
+def true : ObjectId := const 2
+def ellipsis : ObjectId := const 3
+def notImplemented : ObjectId := const 4
 
 def nonScalar (n : NonScalar) : ObjectId :=
-  .mk <| (unsafe ptrAddrUnsafe n).toUInt64
+  mk (unsafe ptrAddrUnsafe n).toUInt64
+
+end ObjectId
+
+@[inline] def IntRef.id (n : IntRef) : ObjectId :=
+  ⟨n.addr.toUInt64⟩
+
+theorem IntRef.id_ne_const : id n ≠ .const c := by
+  rw [ne_eq, ← ObjectId.toNat_inj]
+  if h : n.isSmall then
+    refine Nat.ne_of_lt (Nat.lt_of_lt_of_le ?_ ObjectId.le_toNat_const)
+    simp [id, IntRef.addr_of_isSmall h, toNat_smallIntAddr_lt]
+  else
+    intro h_eq
+    replace h_eq := congrArg (· % 2) h_eq
+    simp [IntRef.toNat_addr_of_not_isSmall h, id] at h_eq
