LeanPy/Util/String.lean
@@ -6,9 +6,6 @@ syntax Authors Mac Malone
 
 namespace LeanPy
 
-def lpad (s : String) (c : Char) (len : Nat) : String :=
-  "".pushn c (len - s.length) ++ s
-
 theorem isValidChar_of_lt_255 (h : n < 255) : isValidChar n := by
   grind
 
@@ -16,22 +13,31 @@ def upperHexChar (n : UInt32) : Char :=
   if h : n ≤ 9 then
     ⟨n + 48, isValidChar_of_lt_255 (by grind)⟩ -- + '0'
   else if h : n ≤ 0xf then
-    ⟨n + 78, isValidChar_of_lt_255 (by grind)⟩ -- + ('a' - 10)
+    ⟨n + 55, isValidChar_of_lt_255 (by grind)⟩ -- + ('A' - 10)
   else
     '*'
 
+-- sanity check
+example : "FEDCBA9876543210" =
+  (String.mk <| (16).fold (init := []) fun i _ s =>
+    upperHexChar i.toUInt32 :: s)
+:= by decide
+
+set_option linter.unusedVariables false in
 def upperHexUInt64 (n : UInt64) : String :=
-  lpad (go n "") '0' 16
+  .mk <| (go n []).leftpad 16 '0'
 where
   go n s :=
     let d := upperHexChar (n % 16).toUInt32
-    let s := s.push d
-    if h : n = 0 then
+    let s := d :: s
+    let n' := n / 16
+    if h : n' = 0 then
       s
     else
-      go (n / 16) s
-  termination_by n
+      go n' s
+  termination_by n.toNat
   decreasing_by
+    simp only [UInt64.toNat_div, UInt64.reduceToNat]
+    refine Nat.div_lt_self (k := 16) ?_ (by simp)
     simp only [← UInt64.toNat_inj, UInt64.toNat_zero] at h
-    replace h := Nat.div_lt_self (k := 16) (Nat.pos_of_ne_zero h) (by simp)
-    simp [h]
+    exact Nat.pos_of_div_pos (Nat.pos_of_ne_zero h)
