LeanPy/Data/IntRef.lean
@@ -1,0 +1,138 @@
+/-
+Copyright (c) 2025 Mac Malone. All rights reserved.
+Released under the Apache 2.0 license as described in the file LICENSE.
+syntax Authors Mac Malone
+-/
+import LeanPy.Util.WithAddr
+
+namespace LeanPy
+
+/-! ## Small Int -/
+
+def smallIntBits : Nat :=
+  if System.Platform.numBits == 64 then 32 else 31
+
+@[inline] unsafe def isScalarUnsafe (a : α) : Bool :=
+  ptrAddrUnsafe a &&& 1 == 1
+
+@[inline] private unsafe def isSmallIntImpl (n : Int) : Bool :=
+  isScalarUnsafe n
+
+@[implemented_by isSmallIntImpl]
+def isSmallInt (n : Int) : Bool :=
+  - 2 ^ (smallIntBits - 1) ≤ n ∧ n ≤ 2 ^ (smallIntBits - 1) - 1
+
+theorem isSmallInt_of_lt (h : n.natAbs < 1073741823) : isSmallInt n := by
+  simp only [isSmallInt, smallIntBits]
+  split <;> grind
+
+theorem isSmallInt_zero : isSmallInt 0 :=
+  isSmallInt_of_lt (by decide)
+
+def smallIntAddr (n : Int) : USize :=
+  n.toInt32.toUInt32.toUSize <<< 1 ||| 1
+
+theorem toNat_smallIntAddr_lt : (smallIntAddr n).toNat < 8589934592 := by
+  have one_mod_numBits : 1 % System.Platform.numBits = 1 :=
+    Nat.mod_eq_of_lt (Nat.lt_of_lt_of_le (by simp) System.Platform.le_numBits)
+  rw [smallIntAddr]
+  simp only [USize.toNat_or, USize.toNat_shiftLeft, USize.reduceToNat]
+  refine Nat.or_lt_two_pow (n := 33) (Nat.mod_lt_of_lt ?_) (by simp)
+  rw [one_mod_numBits, Nat.shiftLeft_eq, Nat.pow_one, UInt32.toNat_toUSize]
+  have n_lt := n.toInt32.toUInt32.toNat_lt
+  omega
+
+@[simp] theorem toNat_smallIntAddr_mod_two : (smallIntAddr n).toNat % 2 = 1 := by
+  simp [smallIntAddr]
+
+@[simp] theorem smallIntAddr_mod_two : smallIntAddr n % 2 = 1 := by
+  simp [← USize.toNat_inj, toNat_smallIntAddr_mod_two]
+
+theorem toNat_smallIntAddr_ne_zero : (smallIntAddr n).toNat ≠ 0 := by
+  simp only [smallIntAddr, USize.toNat_or, USize.reduceToNat]
+  simp only [Nat.ne_zero_iff_zero_lt, Nat.lt_of_succ_le Nat.right_le_or]
+
+theorem smallIntAddr_ne_zero : smallIntAddr n ≠ 0 := by
+  rw [ne_eq, ← USize.toNat_inj, ← ne_eq]
+  exact toNat_smallIntAddr_ne_zero
+
+/-! ## Int Ref -/
+
+abbrev IntRef.WF (n : WithAddr Int) : Prop :=
+  if isSmallInt n.data then n.addr = smallIntAddr n.data else n.addr % 2 = 0
+
+structure IntRef where
+  toWithAddr : WithAddr Int
+  wf : IntRef.WF toWithAddr
+  deriving TypeName
+
+namespace IntRef
+
+@[inline] def addr (n : IntRef) : USize :=
+  n.toWithAddr.addr
+
+@[simp] theorem addr_mk : addr (mk v h) = v.addr := rfl
+
+@[inline] def toInt (n : IntRef) : Int :=
+  n.toWithAddr.data
+
+instance : Coe IntRef Int := ⟨toInt⟩
+
+@[simp] theorem toInt_mk : toInt (mk n h) = n.data := rfl
+
+@[inline] def isSmall (n : IntRef) : Bool :=
+  isSmallInt n.toInt
+
+@[simp] theorem isSmall_mk : isSmall (mk n h) = isSmallInt n.data := rfl
+
+theorem addr_of_isSmall (h : isSmall n) : addr n = smallIntAddr n.toInt := by
+  let ⟨n, wf⟩  := n
+  simp only [isSmall_mk] at h
+  simpa [WF, h] using wf
+
+theorem addr_of_not_isSmall (h : ¬ isSmall n) : addr n % 2 = 0 := by
+  let ⟨n, wf⟩  := n
+  simp only [isSmall_mk] at h
+  simpa [WF, h] using wf
+
+theorem toNat_addr_of_not_isSmall (h : ¬ isSmall n) : (addr n).toNat % 2 = 0 := by
+  simpa [← USize.toNat_inj] using addr_of_not_isSmall h
+
+@[inline] private unsafe def ofSmallIntImpl (n : Int) (_ : isSmallInt n) : IntRef :=
+  unsafeCast n
+
+@[implemented_by ofSmallIntImpl]
+def ofIsSmall (n : Int) (h : isSmallInt n) : IntRef :=
+  ⟨.mk (smallIntAddr n) n, by simp [IntRef.WF, h]⟩
+
+instance : OfNat IntRef 0 := ⟨.ofIsSmall 0 isSmallInt_zero⟩
+
+@[simp] theorem toInt_ofIsSmall : (ofIsSmall n h).toInt = n := rfl
+
+instance : Nonempty IntRef := ⟨.ofIsSmall 0 isSmallInt_zero⟩
+
+@[simp] theorem toInt_zero : toInt 0 = 0 := rfl
+
+private noncomputable def null (n : Int) (h : ¬ isSmallInt n) : IntRef :=
+  ⟨.mk 0 n, by simp [IntRef.WF, h]⟩
+
+private theorem toInt_null : toInt (null n h) = n := rfl
+
+end IntRef
+
+@[noinline] -- prevents compiler from producing incorrect casts
+unsafe def intRefUnsafe (n : Int) : IntRef :=
+ unsafeCast n
+
+@[inline] private unsafe def mkIntRefImpl (n : Int) : BaseIO {r : IntRef // r = n} :=
+ pure ⟨intRefUnsafe n, lcProof⟩
+
+@[implemented_by mkIntRefImpl]
+opaque mkIntRef' (n : Int) : BaseIO {r : IntRef // r = n} := do
+  if h : isSmallInt n then
+    return ⟨.ofIsSmall n h, IntRef.toInt_ofIsSmall⟩
+  else
+    return ⟨IntRef.null n h, IntRef.toInt_null⟩
+
+@[inline] def mkIntRef (n : Int) : BaseIO IntRef :=
+  (·.val) <$> mkIntRef' n
